ExactBacktranslation/AnnotatedGlobalCoercions.v
@@ -1,0 +1,816 @@
+Require Import ExactBacktranslation.CertificateIndexed.
+Require Import ExactBacktranslation.CastCommon.
+Require Import ExactBacktranslation.StructuralCoercions.
+Require Import ExactBacktranslation.GlobalCoercions.
+Require Import StlcIso.SpecAnnot.
+Require Import StlcIso.InstAnnot.
+Require Import StlcIso.Fix.
+Require Import StlcIso.LemmasTyping.
+From Coq Require Import Lists.List.
+From Coq Require Import Logic.FunctionalExtensionality.
+Import ListNotations.
+
+Module IA := StlcIso.SpecAnnot.
+
+(** A computationally annotated counterpart of the heterogeneous environment
+    used by the raw global coercion interpreter. *)
+Fixpoint CastTermsA (H : PairEnv) : Type :=
+  match H with
+  | nil => Datatypes.unit
+  | _ :: H' => (IA.TmA * CastTermsA H')%type
+  end.
+
+Definition cast_terms_annot_nil : CastTermsA nil := tt.
+
+Definition cast_terms_annot_cons {H A B}
+  (t : IA.TmA) (rho : CastTermsA H) : CastTermsA ((A, B) :: H) :=
+  (t, rho).
+
+Fixpoint erase_cast_terms_annot {H} : CastTermsA H -> CastTerms H :=
+  match H return CastTermsA H -> CastTerms H with
+  | nil => fun _ => tt
+  | _ :: H' => fun rho =>
+      (IA.eraseAnnot (fst rho), erase_cast_terms_annot (snd rho))
+  end.
+
+Fixpoint lookup_cast_annot {H A B}
+  (m : Assumed H A B) : CastTermsA H -> IA.TmA :=
+  match m with
+  | assumed_here => fun rho => fst rho
+  | assumed_there m' => fun rho => lookup_cast_annot m' (snd rho)
+  end.
+
+Lemma erase_lookup_cast_annot {H A B} (m : Assumed H A B)
+    (rho : CastTermsA H) :
+  IA.eraseAnnot (lookup_cast_annot m rho) =
+  lookup_cast m (erase_cast_terms_annot rho).
+Proof. induction m; cbn; auto. Qed.
+
+Definition pair_up_annot (A B : Ty) (p : IA.TmA) : IA.TmA :=
+  IA.ia_proj₁ (tarr A B) (tarr B A) p.
+
+Definition pair_down_annot (A B : Ty) (p : IA.TmA) : IA.TmA :=
+  IA.ia_proj₂ (tarr A B) (tarr B A) p.
+
+Definition certificate_root_annot {H A B} (d : CastEq H A B)
+    (self : IA.TmA) (rho : CastTermsA H) : IA.TmA :=
+  match d in CastEq H0 A0 B0
+        return IA.TmA -> CastTermsA H0 -> IA.TmA with
+  | @ce_back H0 A0 B0 m => fun _ rho0 => lookup_cast_annot m rho0
+  | @ce_step H0 A0 B0 node => fun self0 _ =>
+      IA.ia_proj₁ (cast_pair_ty A0 B0) (node_bundle_ty node) self0
+  end self rho.
+
+Definition certificate_up_annot {H A B} (d : CastEq H A B)
+    (self : IA.TmA) (rho : CastTermsA H) : IA.TmA :=
+  pair_up_annot A B (certificate_root_annot d self rho).
+
+Definition certificate_down_annot {H A B} (d : CastEq H A B)
+    (self : IA.TmA) (rho : CastTermsA H) : IA.TmA :=
+  pair_down_annot A B (certificate_root_annot d self rho).
+
+(** Every ordinary fold/unfold introduced by the raw interpreter is annotated
+    here with the recursive body supplied by the corresponding certificate
+    node. *)
+Definition global_node_cast_annot {H A B} (node : CastNode H A B)
+    (payload_self : IA.TmA)
+    (rho : CastTermsA ((A, B) :: H)) : IA.TmA :=
+  match node in CastNode H0 A0 B0
+        return IA.TmA -> CastTermsA ((A0, B0) :: H0) -> IA.TmA with
+  | cn_unit _ => fun _ _ =>
+      IA.ia_pair (tarr tunit tunit) (tarr tunit tunit)
+        (IA.ia_abs tunit tunit (IA.ia_var 0))
+        (IA.ia_abs tunit tunit (IA.ia_var 0))
+  | cn_bool _ => fun _ _ =>
+      IA.ia_pair (tarr tbool tbool) (tarr tbool tbool)
+        (IA.ia_abs tbool tbool (IA.ia_var 0))
+        (IA.ia_abs tbool tbool (IA.ia_var 0))
+  | cn_var _ x => fun _ _ =>
+      IA.ia_pair (tarr (tvar x) (tvar x)) (tarr (tvar x) (tvar x))
+        (IA.ia_abs (tvar x) (tvar x) (IA.ia_var 0))
+        (IA.ia_abs (tvar x) (tvar x) (IA.ia_var 0))
+  | cn_arr _ A1 A2 B1 B2 dom cod => fun ps rho0 =>
+      let dp := certificate_root_annot dom
+        (IA.ia_proj₁ (certificate_bundle_ty dom)
+          (certificate_bundle_ty cod) ps) rho0 in
+      let cp := certificate_root_annot cod
+        (IA.ia_proj₂ (certificate_bundle_ty dom)
+          (certificate_bundle_ty cod) ps) rho0 in
+      IA.ia_pair
+        (tarr (tarr A1 A2) (tarr B1 B2))
+        (tarr (tarr B1 B2) (tarr A1 A2))
+        (IA.ia_abs (tarr A1 A2) (tarr B1 B2)
+          (IA.ia_abs B1 B2
+            (IA.ia_app A2 B2 (pair_up_annot A2 B2 cp)[wkm][wkm]
+              (IA.ia_app A1 A2 (IA.ia_var 1)
+                (IA.ia_app B1 A1
+                  (pair_down_annot A1 B1 dp)[wkm][wkm]
+                  (IA.ia_var 0))))))
+        (IA.ia_abs (tarr B1 B2) (tarr A1 A2)
+          (IA.ia_abs A1 A2
+            (IA.ia_app B2 A2 (pair_down_annot A2 B2 cp)[wkm][wkm]
+              (IA.ia_app B1 B2 (IA.ia_var 1)
+                (IA.ia_app A1 B1
+                  (pair_up_annot A1 B1 dp)[wkm][wkm]
+                  (IA.ia_var 0))))))
+  | cn_prod _ A1 A2 B1 B2 fstc sndc => fun ps rho0 =>
+      let fp := certificate_root_annot fstc
+        (IA.ia_proj₁ (certificate_bundle_ty fstc)
+          (certificate_bundle_ty sndc) ps) rho0 in
+      let sp := certificate_root_annot sndc
+        (IA.ia_proj₂ (certificate_bundle_ty fstc)
+          (certificate_bundle_ty sndc) ps) rho0 in
+      IA.ia_pair
+        (tarr (tprod A1 A2) (tprod B1 B2))
+        (tarr (tprod B1 B2) (tprod A1 A2))
+        (IA.ia_abs (tprod A1 A2) (tprod B1 B2)
+          (IA.ia_pair B1 B2
+            (IA.ia_app A1 B1 (pair_up_annot A1 B1 fp)[wkm]
+              (IA.ia_proj₁ A1 A2 (IA.ia_var 0)))
+            (IA.ia_app A2 B2 (pair_up_annot A2 B2 sp)[wkm]
+              (IA.ia_proj₂ A1 A2 (IA.ia_var 0)))))
+        (IA.ia_abs (tprod B1 B2) (tprod A1 A2)
+          (IA.ia_pair A1 A2
+            (IA.ia_app B1 A1 (pair_down_annot A1 B1 fp)[wkm]
+              (IA.ia_proj₁ B1 B2 (IA.ia_var 0)))
+            (IA.ia_app B2 A2 (pair_down_annot A2 B2 sp)[wkm]
+              (IA.ia_proj₂ B1 B2 (IA.ia_var 0)))))
+  | cn_sum _ A1 A2 B1 B2 lc rc => fun ps rho0 =>
+      let lp := certificate_root_annot lc
+        (IA.ia_proj₁ (certificate_bundle_ty lc)
+          (certificate_bundle_ty rc) ps) rho0 in
+      let rp := certificate_root_annot rc
+        (IA.ia_proj₂ (certificate_bundle_ty lc)
+          (certificate_bundle_ty rc) ps) rho0 in
+      IA.ia_pair
+        (tarr (tsum A1 A2) (tsum B1 B2))
+        (tarr (tsum B1 B2) (tsum A1 A2))
+        (IA.ia_abs (tsum A1 A2) (tsum B1 B2)
+          (IA.ia_caseof A1 A2 (tsum B1 B2) (IA.ia_var 0)
+            (IA.ia_inl B1 B2
+              (IA.ia_app A1 B1 (pair_up_annot A1 B1 lp)[wkm][wkm]
+                (IA.ia_var 0)))
+            (IA.ia_inr B1 B2
+              (IA.ia_app A2 B2 (pair_up_annot A2 B2 rp)[wkm][wkm]
+                (IA.ia_var 0)))))
+        (IA.ia_abs (tsum B1 B2) (tsum A1 A2)
+          (IA.ia_caseof B1 B2 (tsum A1 A2) (IA.ia_var 0)
+            (IA.ia_inl A1 A2
+              (IA.ia_app B1 A1 (pair_down_annot A1 B1 lp)[wkm][wkm]
+                (IA.ia_var 0)))
+            (IA.ia_inr A1 A2
+              (IA.ia_app B2 A2 (pair_down_annot A2 B2 rp)[wkm][wkm]
+                (IA.ia_var 0)))))
+  | cn_mu_l _ body B child => fun ps rho0 =>
+      let cp := certificate_root_annot child ps rho0 in
+      IA.ia_pair
+        (tarr (trec body) B) (tarr B (trec body))
+        (IA.ia_abs (trec body) B
+          (IA.ia_app body[beta1 (trec body)] B
+            (pair_up_annot body[beta1 (trec body)] B cp)[wkm]
+            (IA.ia_unfold_ body (IA.ia_var 0))))
+        (IA.ia_abs B (trec body)
+          (IA.ia_fold_ body
+            (IA.ia_app B body[beta1 (trec body)]
+              (pair_down_annot body[beta1 (trec body)] B cp)[wkm]
+              (IA.ia_var 0))))
+  | cn_mu_r _ A body _ child => fun ps rho0 =>
+      let cp := certificate_root_annot child ps rho0 in
+      IA.ia_pair
+        (tarr A (trec body)) (tarr (trec body) A)
+        (IA.ia_abs A (trec body)
+          (IA.ia_fold_ body
+            (IA.ia_app A body[beta1 (trec body)]
+              (pair_up_annot A body[beta1 (trec body)] cp)[wkm]
+              (IA.ia_var 0))))
+        (IA.ia_abs (trec body) A
+          (IA.ia_app body[beta1 (trec body)] A
+            (pair_down_annot A body[beta1 (trec body)] cp)[wkm]
+            (IA.ia_unfold_ body (IA.ia_var 0))))
+  end payload_self rho.
+
+Fixpoint build_certificate_bundle_annot {H A B} (d : CastEq H A B)
+    (self : IA.TmA) (rho : CastTermsA H) {struct d} : IA.TmA :=
+  match d in CastEq H0 A0 B0
+        return IA.TmA -> CastTermsA H0 -> IA.TmA with
+  | @ce_back H0 A0 B0 _ => fun _ _ => IA.ia_unit
+  | @ce_step H0 A0 B0 node => fun self0 rho0 =>
+      let root_self := IA.ia_proj₁ (cast_pair_ty A0 B0)
+        (node_bundle_ty node) self0 in
+      let payload_self := IA.ia_proj₂ (cast_pair_ty A0 B0)
+        (node_bundle_ty node) self0 in
+      let rho' := cast_terms_annot_cons root_self rho0 in
+      IA.ia_pair (cast_pair_ty A0 B0) (node_bundle_ty node)
+        (global_node_cast_annot node payload_self rho')
+        (build_node_bundle_annot node payload_self rho')
+  end self rho
+with build_node_bundle_annot {H A B} (node : CastNode H A B)
+    (payload_self : IA.TmA)
+    (rho : CastTermsA ((A, B) :: H)) {struct node} : IA.TmA :=
+  match node in CastNode H0 A0 B0
+        return IA.TmA -> CastTermsA ((A0, B0) :: H0) -> IA.TmA with
+  | cn_unit _ | cn_bool _ | cn_var _ _ => fun _ _ => IA.ia_unit
+  | cn_arr _ _ _ _ _ l r
+  | cn_prod _ _ _ _ _ l r
+  | cn_sum _ _ _ _ _ l r => fun ps rho0 =>
+      IA.ia_pair (certificate_bundle_ty l) (certificate_bundle_ty r)
+        (build_certificate_bundle_annot l
+          (IA.ia_proj₁ (certificate_bundle_ty l)
+            (certificate_bundle_ty r) ps) rho0)
+        (build_certificate_bundle_annot r
+          (IA.ia_proj₂ (certificate_bundle_ty l)
+            (certificate_bundle_ty r) ps) rho0)
+  | cn_mu_l _ _ _ child => fun ps rho0 =>
+      build_certificate_bundle_annot child ps rho0
+  | cn_mu_r _ _ _ _ child => fun ps rho0 =>
+      build_certificate_bundle_annot child ps rho0
+  end payload_self rho.
+
+Definition global_bundle_functional_annot {A B}
+    (d : ClosedCastEq A B) : IA.TmA :=
+  let BT := certificate_bundle_ty d in
+  let self := IA.ia_app tunit BT (IA.ia_var 1) IA.ia_unit in
+  IA.ia_abs (tarr tunit BT) (tarr tunit BT)
+    (IA.ia_abs tunit BT
+      (build_certificate_bundle_annot d self cast_terms_annot_nil)).
+
+Definition tied_certificate_bundle_annot {A B}
+    (d : ClosedCastEq A B) : IA.TmA :=
+  let BT := certificate_bundle_ty d in
+  IA.ia_app tunit BT
+    (IA.ia_app
+      (tarr (tarr tunit BT) (tarr tunit BT))
+      (tarr tunit BT)
+      (ufix_annot tunit BT) (global_bundle_functional_annot d))
+    IA.ia_unit.
+
+Definition compile_global_pair_annot {A B}
+    (d : ClosedCastEq A B) : IA.TmA :=
+  certificate_root_annot d (tied_certificate_bundle_annot d)
+    cast_terms_annot_nil.
+
+Definition compile_global_up_annot {A B}
+    (d : ClosedCastEq A B) : IA.TmA :=
+  pair_up_annot A B (compile_global_pair_annot d).
+
+Definition compile_global_down_annot {A B}
+    (d : ClosedCastEq A B) : IA.TmA :=
+  pair_down_annot A B (compile_global_pair_annot d).
+
+(** Erasure commutes with the renamings used inside generated casts. *)
+Lemma erase_annot_ren (t : IA.TmA) (xi : Sub Ix) :
+  IA.eraseAnnot (IA.apTmA xi t) =
+  StlcIso.SpecSyntax.apTm xi (IA.eraseAnnot t).
+Proof. revert xi. induction t; intros xi; cbn; f_equal; eauto. Qed.
+
+Lemma erase_annot_var_sub (t : IA.TmA) (xi : Sub Ix) :
+  IA.eraseAnnot (IA.apTmA (fun x => IA.ia_var (xi x)) t) =
+  StlcIso.SpecSyntax.apTm
+    (fun x => StlcIso.SpecSyntax.var (xi x)) (IA.eraseAnnot t).
+Proof.
+  assert (HA : forall zeta : Sub Ix,
+    (fun x => IA.ia_var (zeta x))↑ =
+    (fun x => IA.ia_var ((zeta↑) x))).
+  { intros zeta. apply functional_extensionality.
+    intros [|x]; reflexivity. }
+  assert (HI : forall zeta : Sub Ix,
+    (fun x => StlcIso.SpecSyntax.var (zeta x))↑ =
+    (fun x => StlcIso.SpecSyntax.var ((zeta↑) x))).
+  { intros zeta. apply functional_extensionality.
+    intros [|x]; reflexivity. }
+  revert xi. induction t; intros xi; cbn;
+    repeat rewrite HA; repeat rewrite HI; f_equal; eauto.
+Qed.
+
+Lemma erase_annot_wkm (t : IA.TmA) :
+  IA.eraseAnnot (IA.apTmA wkm t) =
+  StlcIso.SpecSyntax.apTm wkm (IA.eraseAnnot t).
+Proof.
+  change (IA.eraseAnnot
+    (IA.apTmA (fun x => IA.ia_var (S x)) t) =
+    StlcIso.SpecSyntax.apTm
+      (fun x => StlcIso.SpecSyntax.var (S x)) (IA.eraseAnnot t)).
+  exact (erase_annot_var_sub t (fun x => S x)).
+Qed.
+
+Lemma erase_certificate_root_annot {H A B} (d : CastEq H A B)
+    self (rho : CastTermsA H) :
+  IA.eraseAnnot (certificate_root_annot d self rho) =
+  certificate_root d (IA.eraseAnnot self) (erase_cast_terms_annot rho).
+Proof.
+  destruct d; cbn; auto using erase_lookup_cast_annot.
+Qed.
+
+Lemma erase_global_node_cast_annot {H A B} (node : CastNode H A B)
+    payload (rho : CastTermsA ((A, B) :: H)) :
+  IA.eraseAnnot (global_node_cast_annot node payload rho) =
+  global_node_cast node (IA.eraseAnnot payload)
+    (erase_cast_terms_annot rho).
+Proof.
+  destruct node; cbn;
+    repeat rewrite erase_annot_wkm;
+    repeat setoid_rewrite erase_certificate_root_annot;
+    reflexivity.
+Qed.
+
+Lemma erase_build_certificate_bundle_annot {H A B}
+    (d : CastEq H A B) self (rho : CastTermsA H) :
+  IA.eraseAnnot (build_certificate_bundle_annot d self rho) =
+  build_certificate_bundle d (IA.eraseAnnot self)
+    (erase_cast_terms_annot rho)
+with erase_build_node_bundle_annot {H A B}
+    (node : CastNode H A B) payload
+    (rho : CastTermsA ((A, B) :: H)) :
+  IA.eraseAnnot (build_node_bundle_annot node payload rho) =
+  build_node_bundle node (IA.eraseAnnot payload)
+    (erase_cast_terms_annot rho).
+Proof.
+  - destruct d; cbn -[global_node_cast_annot global_node_cast
+      build_node_bundle_annot build_node_bundle].
+    + reflexivity.
+    + rewrite erase_global_node_cast_annot.
+      rewrite erase_build_node_bundle_annot.
+      reflexivity.
+  - destruct node; cbn -[build_certificate_bundle_annot
+      build_certificate_bundle]; try reflexivity;
+      repeat rewrite erase_build_certificate_bundle_annot; reflexivity.
+Qed.
+
+Theorem erase_global_bundle_functional_annot {A B}
+    (d : ClosedCastEq A B) :
+  IA.eraseAnnot (global_bundle_functional_annot d) =
+  global_bundle_functional d.
+Proof.
+  unfold global_bundle_functional_annot, global_bundle_functional.
+  cbn. now rewrite erase_build_certificate_bundle_annot.
+Qed.
+
+Theorem erase_tied_certificate_bundle_annot {A B}
+    (d : ClosedCastEq A B) :
+  IA.eraseAnnot (tied_certificate_bundle_annot d) =
+  tied_certificate_bundle d.
+Proof.
+  unfold tied_certificate_bundle_annot, tied_certificate_bundle.
+  cbn -[ufix_annot global_bundle_functional_annot].
+  rewrite eraseAnnot_ufix, erase_global_bundle_functional_annot.
+  reflexivity.
+Qed.
+
+Theorem erase_compile_global_pair_annot {A B}
+    (d : ClosedCastEq A B) :
+  IA.eraseAnnot (compile_global_pair_annot d) = compile_global_pair d.
+Proof.
+  unfold compile_global_pair_annot, compile_global_pair.
+  rewrite erase_certificate_root_annot.
+  now rewrite erase_tied_certificate_bundle_annot.
+Qed.
+
+Theorem erase_compile_global_up_annot {A B}
+    (d : ClosedCastEq A B) :
+  IA.eraseAnnot (compile_global_up_annot d) = compile_global_up d.
+Proof.
+  unfold compile_global_up_annot, compile_global_up, pair_up_annot, pair_up.
+  cbn. now rewrite erase_compile_global_pair_annot.
+Qed.
+
+Theorem erase_compile_global_down_annot {A B}
+    (d : ClosedCastEq A B) :
+  IA.eraseAnnot (compile_global_down_annot d) = compile_global_down d.
+Proof.
+  unfold compile_global_down_annot, compile_global_down,
+    pair_down_annot, pair_down.
+  cbn. now rewrite erase_compile_global_pair_annot.
+Qed.
+
+(** Direct annotated typing: this does not reify a raw typing derivation in
+    [Prop]. *)
+Lemma annot_typing_var_ren {Gamma1 t T} :
+  IA.AnnotTyping Gamma1 t T ->
+  forall Gamma2 (xi : Sub Ix), WtRen Gamma1 Gamma2 xi ->
+  IA.AnnotTyping Gamma2
+    (IA.apTmA (fun x => IA.ia_var (xi x)) t) T.
+Proof.
+  intros Ht.
+  assert (HA : forall zeta : Sub Ix,
+    (fun x => IA.ia_var (zeta x))↑ =
+    (fun x => IA.ia_var ((zeta↑) x))).
+  { intros zeta. apply functional_extensionality.
+    intros [|x]; reflexivity. }
+  induction Ht; intros Gamma2 xi Hxi; cbn;
+    repeat rewrite HA; eauto using IA.AnnotTyping, wtRen_up.
+  econstructor; eauto using wtRen_up.
+Qed.
+
+Lemma annot_typing_weaken {Gamma t T U} :
+  IA.AnnotTyping Gamma t T ->
+  IA.AnnotTyping (Gamma r▻ U) t[wkm] T.
+Proof.
+  intros Ht.
+  change (IA.AnnotTyping (Gamma r▻ U)
+    (IA.apTmA (fun x => IA.ia_var (S x)) t) T).
+  eapply annot_typing_var_ren; [exact Ht|apply wtRen_wkm].
+Qed.
+
+Fixpoint CastTermsATyping (Gamma : Env) (H : PairEnv) :
+    CastTermsA H -> Prop :=
+  match H return CastTermsA H -> Prop with
+  | nil => fun _ => True
+  | (A, B) :: H' => fun rho =>
+      IA.AnnotTyping Gamma (fst rho) (cast_pair_ty A B) /\
+      CastTermsATyping Gamma H' (snd rho)
+  end.
+
+Lemma cast_terms_annot_typing_nil Gamma :
+  CastTermsATyping Gamma nil cast_terms_annot_nil.
+Proof. exact I. Qed.
+
+Lemma cast_terms_annot_typing_cons {H A B Gamma t rho} :
+  IA.AnnotTyping Gamma t (cast_pair_ty A B) ->
+  CastTermsATyping Gamma H rho ->
+  CastTermsATyping Gamma ((A, B) :: H)
+    (cast_terms_annot_cons t rho).
+Proof. split; assumption. Qed.
+
+Lemma lookup_cast_annot_typing {Gamma H A B}
+    (m : Assumed H A B) rho :
+  CastTermsATyping Gamma H rho ->
+  IA.AnnotTyping Gamma (lookup_cast_annot m rho) (cast_pair_ty A B).
+Proof.
+  revert rho. induction m; intros rho Hrho; cbn in *.
+  - exact (proj1 Hrho).
+  - apply IHm. exact (proj2 Hrho).
+Qed.
+
+Lemma pair_up_annot_typing {Gamma p A B} :
+  IA.AnnotTyping Gamma p (cast_pair_ty A B) ->
+  IA.AnnotTyping Gamma (pair_up_annot A B p) (tarr A B).
+Proof.
+  intros Hp. unfold pair_up_annot, cast_pair_ty in *.
+  now apply IA.ia_WtProj1.
+Qed.
+
+Lemma pair_down_annot_typing {Gamma p A B} :
+  IA.AnnotTyping Gamma p (cast_pair_ty A B) ->
+  IA.AnnotTyping Gamma (pair_down_annot A B p) (tarr B A).
+Proof.
+  intros Hp. unfold pair_down_annot, cast_pair_ty in *.
+  now apply IA.ia_WtProj2.
+Qed.
+
+Lemma certificate_root_annot_typing {Gamma H A B}
+    (d : CastEq H A B) self rho :
+  IA.AnnotTyping Gamma self (certificate_bundle_ty d) ->
+  CastTermsATyping Gamma H rho ->
+  IA.AnnotTyping Gamma (certificate_root_annot d self rho)
+    (cast_pair_ty A B).
+Proof.
+  destruct d; cbn; intros Hself Hrho.
+  - now apply lookup_cast_annot_typing.
+  - apply IA.ia_WtProj1. exact Hself.
+Qed.
+
+Lemma certificate_up_annot_typing {Gamma H A B}
+    (d : CastEq H A B) self rho :
+  IA.AnnotTyping Gamma self (certificate_bundle_ty d) ->
+  CastTermsATyping Gamma H rho ->
+  IA.AnnotTyping Gamma (certificate_up_annot d self rho) (tarr A B).
+Proof.
+  intros Hself Hrho. apply pair_up_annot_typing.
+  now apply certificate_root_annot_typing.
+Qed.
+
+Lemma certificate_down_annot_typing {Gamma H A B}
+    (d : CastEq H A B) self rho :
+  IA.AnnotTyping Gamma self (certificate_bundle_ty d) ->
+  CastTermsATyping Gamma H rho ->
+  IA.AnnotTyping Gamma (certificate_down_annot d self rho) (tarr B A).
+Proof.
+  intros Hself Hrho. apply pair_down_annot_typing.
+  now apply certificate_root_annot_typing.
+Qed.
+
+Lemma id_cast_annot_typing {Gamma A} :
+  ValidTy A ->
+  IA.AnnotTyping Gamma (IA.ia_abs A A (IA.ia_var 0)) (tarr A A).
+Proof.
+  intros VA. apply IA.ia_WtAbs; [exact VA|].
+  apply IA.ia_WtVar. constructor.
+Qed.
+
+Lemma global_node_cast_annot_typing {Gamma H A B}
+    (node : CastNode H A B) payload_self rho :
+  PairEnvValid H -> ValidTy A -> ValidTy B ->
+  IA.AnnotTyping Gamma payload_self (node_bundle_ty node) ->
+  CastTermsATyping Gamma ((A, B) :: H) rho ->
+  IA.AnnotTyping Gamma (global_node_cast_annot node payload_self rho)
+    (cast_pair_ty A B).
+Proof.
+  destruct node as
+      [H|H|H x
+      |H A1 A2 B1 B2 dom cod
+      |H A1 A2 B1 B2 fstc sndc
+      |H A1 A2 B1 B2 lc rc
+      |H body B child
+      |H A body nmu child]; intros VH VA VB Hself Hrho; cbn in *.
+  - apply IA.ia_WtPair; apply id_cast_annot_typing; assumption.
+  - apply IA.ia_WtPair; apply id_cast_annot_typing; assumption.
+  - apply IA.ia_WtPair; apply id_cast_annot_typing; assumption.
+  - apply ValidTy_invert_arr in VA as [VA1 VA2].
+    apply ValidTy_invert_arr in VB as [VB1 VB2].
+    assert (Hdomself : IA.AnnotTyping Gamma
+      (IA.ia_proj₁ (certificate_bundle_ty dom)
+        (certificate_bundle_ty cod) payload_self)
+      (certificate_bundle_ty dom))
+      by (apply IA.ia_WtProj1; exact Hself).
+    assert (Hcodself : IA.AnnotTyping Gamma
+      (IA.ia_proj₂ (certificate_bundle_ty dom)
+        (certificate_bundle_ty cod) payload_self)
+      (certificate_bundle_ty cod))
+      by (apply IA.ia_WtProj2; exact Hself).
+    assert (Hdom := certificate_root_annot_typing dom _ _ Hdomself Hrho).
+    assert (Hcod := certificate_root_annot_typing cod _ _ Hcodself Hrho).
+    assert (HUdom := pair_up_annot_typing Hdom).
+    assert (HDdom := pair_down_annot_typing Hdom).
+    assert (HUcod := pair_up_annot_typing Hcod).
+    assert (HDcod := pair_down_annot_typing Hcod).
+    apply IA.ia_WtPair.
+    + apply IA.ia_WtAbs; [now apply ValidTy_arr|].
+      apply IA.ia_WtAbs; [exact VB1|].
+      eapply IA.ia_WtApp.
+      * exact (annot_typing_weaken
+          (annot_typing_weaken HUcod)).
+      * eapply IA.ia_WtApp.
+        -- apply IA.ia_WtVar. constructor. constructor.
+        -- eapply IA.ia_WtApp.
+           ++ exact (annot_typing_weaken
+                (annot_typing_weaken HDdom)).
+           ++ apply IA.ia_WtVar. constructor.
+    + apply IA.ia_WtAbs; [now apply ValidTy_arr|].
+      apply IA.ia_WtAbs; [exact VA1|].
+      eapply IA.ia_WtApp.
+      * exact (annot_typing_weaken
+          (annot_typing_weaken HDcod)).
+      * eapply IA.ia_WtApp.
+        -- apply IA.ia_WtVar. constructor. constructor.
+        -- eapply IA.ia_WtApp.
+           ++ exact (annot_typing_weaken
+                (annot_typing_weaken HUdom)).
+           ++ apply IA.ia_WtVar. constructor.
+  - apply ValidTy_invert_prod in VA as [VA1 VA2].
+    apply ValidTy_invert_prod in VB as [VB1 VB2].
+    assert (Hfstself : IA.AnnotTyping Gamma
+      (IA.ia_proj₁ (certificate_bundle_ty fstc)
+        (certificate_bundle_ty sndc) payload_self)
+      (certificate_bundle_ty fstc))
+      by (apply IA.ia_WtProj1; exact Hself).
+    assert (Hsndself : IA.AnnotTyping Gamma
+      (IA.ia_proj₂ (certificate_bundle_ty fstc)
+        (certificate_bundle_ty sndc) payload_self)
+      (certificate_bundle_ty sndc))
+      by (apply IA.ia_WtProj2; exact Hself).
+    assert (Hfst := certificate_root_annot_typing fstc _ _ Hfstself Hrho).
+    assert (Hsnd := certificate_root_annot_typing sndc _ _ Hsndself Hrho).
+    assert (HUfst := pair_up_annot_typing Hfst).
+    assert (HDfst := pair_down_annot_typing Hfst).
+    assert (HUsnd := pair_up_annot_typing Hsnd).
+    assert (HDsnd := pair_down_annot_typing Hsnd).
+    apply IA.ia_WtPair.
+    + apply IA.ia_WtAbs; [now apply ValidTy_prod|].
+      apply IA.ia_WtPair.
+      * eapply IA.ia_WtApp; [exact (annot_typing_weaken HUfst)|].
+        apply IA.ia_WtProj1. apply IA.ia_WtVar. constructor.
+      * eapply IA.ia_WtApp; [exact (annot_typing_weaken HUsnd)|].
+        apply IA.ia_WtProj2. apply IA.ia_WtVar. constructor.
+    + apply IA.ia_WtAbs; [now apply ValidTy_prod|].
+      apply IA.ia_WtPair.
+      * eapply IA.ia_WtApp; [exact (annot_typing_weaken HDfst)|].
+        apply IA.ia_WtProj1. apply IA.ia_WtVar. constructor.
+      * eapply IA.ia_WtApp; [exact (annot_typing_weaken HDsnd)|].
+        apply IA.ia_WtProj2. apply IA.ia_WtVar. constructor.
+  - apply ValidTy_invert_sum in VA as [VA1 VA2].
+    apply ValidTy_invert_sum in VB as [VB1 VB2].
+    assert (Hlself : IA.AnnotTyping Gamma
+      (IA.ia_proj₁ (certificate_bundle_ty lc)
+        (certificate_bundle_ty rc) payload_self)
+      (certificate_bundle_ty lc))
+      by (apply IA.ia_WtProj1; exact Hself).
+    assert (Hrself : IA.AnnotTyping Gamma
+      (IA.ia_proj₂ (certificate_bundle_ty lc)
+        (certificate_bundle_ty rc) payload_self)
+      (certificate_bundle_ty rc))
+      by (apply IA.ia_WtProj2; exact Hself).
+    assert (Hl := certificate_root_annot_typing lc _ _ Hlself Hrho).
+    assert (Hr := certificate_root_annot_typing rc _ _ Hrself Hrho).
+    assert (HUl := pair_up_annot_typing Hl).
+    assert (HDl := pair_down_annot_typing Hl).
+    assert (HUr := pair_up_annot_typing Hr).
+    assert (HDr := pair_down_annot_typing Hr).
+    apply IA.ia_WtPair.
+    + apply IA.ia_WtAbs; [now apply ValidTy_sum|].
+      eapply IA.ia_WtCaseof; eauto.
+      * apply IA.ia_WtVar. constructor.
+      * apply IA.ia_WtInl; [exact VB2|].
+        eapply IA.ia_WtApp.
+        -- exact (annot_typing_weaken (annot_typing_weaken HUl)).
+        -- apply IA.ia_WtVar. constructor.
+      * apply IA.ia_WtInr; [exact VB1|].
+        eapply IA.ia_WtApp.
+        -- exact (annot_typing_weaken (annot_typing_weaken HUr)).
+        -- apply IA.ia_WtVar. constructor.
+    + apply IA.ia_WtAbs; [now apply ValidTy_sum|].
+      eapply IA.ia_WtCaseof; eauto.
+      * apply IA.ia_WtVar. constructor.
+      * apply IA.ia_WtInl; [exact VA2|].
+        eapply IA.ia_WtApp.
+        -- exact (annot_typing_weaken (annot_typing_weaken HDl)).
+        -- apply IA.ia_WtVar. constructor.
+      * apply IA.ia_WtInr; [exact VA1|].
+        eapply IA.ia_WtApp.
+        -- exact (annot_typing_weaken (annot_typing_weaken HDr)).
+        -- apply IA.ia_WtVar. constructor.
+  - assert (Hchild := certificate_root_annot_typing
+      child payload_self rho Hself Hrho).
+    assert (HU := pair_up_annot_typing Hchild).
+    assert (HD := pair_down_annot_typing Hchild).
+    apply IA.ia_WtPair.
+    + apply IA.ia_WtAbs; [exact VA|].
+      eapply IA.ia_WtApp.
+      * exact (annot_typing_weaken HU).
+      * apply IA.ia_WtUnfold; [apply IA.ia_WtVar; constructor|exact VA].
+    + apply IA.ia_WtAbs; [exact VB|].
+      apply IA.ia_WtFold; [|exact VA].
+      eapply IA.ia_WtApp; [exact (annot_typing_weaken HD)|].
+      apply IA.ia_WtVar. constructor.
+  - assert (Hchild := certificate_root_annot_typing
+      child payload_self rho Hself Hrho).
+    assert (HU := pair_up_annot_typing Hchild).
+    assert (HD := pair_down_annot_typing Hchild).
+    apply IA.ia_WtPair.
+    + apply IA.ia_WtAbs; [exact VA|].
+      apply IA.ia_WtFold; [|exact VB].
+      eapply IA.ia_WtApp; [exact (annot_typing_weaken HU)|].
+      apply IA.ia_WtVar. constructor.
+    + apply IA.ia_WtAbs; [exact VB|].
+      eapply IA.ia_WtApp.
+      * exact (annot_typing_weaken HD).
+      * apply IA.ia_WtUnfold; [apply IA.ia_WtVar; constructor|exact VB].
+Qed.
+
+Lemma build_certificate_bundle_annot_typing {Gamma H A B}
+    (d : CastEq H A B) self rho :
+  PairEnvValid H -> ValidTy A -> ValidTy B ->
+  IA.AnnotTyping Gamma self (certificate_bundle_ty d) ->
+  CastTermsATyping Gamma H rho ->
+  IA.AnnotTyping Gamma (build_certificate_bundle_annot d self rho)
+    (certificate_bundle_ty d)
+with build_node_bundle_annot_typing {Gamma H A B}
+    (node : CastNode H A B) payload_self rho :
+  PairEnvValid H -> ValidTy A -> ValidTy B ->
+  IA.AnnotTyping Gamma payload_self (node_bundle_ty node) ->
+  CastTermsATyping Gamma ((A, B) :: H) rho ->
+  IA.AnnotTyping Gamma
+    (build_node_bundle_annot node payload_self rho)
+    (node_bundle_ty node).
+Proof.
+  - destruct d as [H A B m|H A B node];
+      intros VH VA VB Hself Hrho; cbn.
+    + apply IA.ia_WtUnit.
+    + assert (Hroot : IA.AnnotTyping Gamma
+        (IA.ia_proj₁ (cast_pair_ty A B) (node_bundle_ty node) self)
+        (cast_pair_ty A B))
+        by (apply IA.ia_WtProj1; exact Hself).
+      assert (Hpayload : IA.AnnotTyping Gamma
+        (IA.ia_proj₂ (cast_pair_ty A B) (node_bundle_ty node) self)
+        (node_bundle_ty node))
+        by (apply IA.ia_WtProj2; exact Hself).
+      assert (Hrho' : CastTermsATyping Gamma ((A, B) :: H)
+        (cast_terms_annot_cons
+          (IA.ia_proj₁ (cast_pair_ty A B) (node_bundle_ty node) self)
+          rho)).
+      { now apply cast_terms_annot_typing_cons. }
+      apply IA.ia_WtPair.
+      * eapply global_node_cast_annot_typing; eauto.
+      * eapply build_node_bundle_annot_typing; eauto.
+  - destruct node as
+      [H|H|H x
+      |H A1 A2 B1 B2 l r
+      |H A1 A2 B1 B2 l r
+      |H A1 A2 B1 B2 l r
+      |H body B child
+      |H A body nmu child]; intros VH VA VB Hself Hrho; cbn in *.
+    + apply IA.ia_WtUnit.
+    + apply IA.ia_WtUnit.
+    + apply IA.ia_WtUnit.
+    + apply ValidTy_invert_arr in VA as [VA1 VA2].
+      apply ValidTy_invert_arr in VB as [VB1 VB2].
+      assert (VH' : PairEnvValid ((tarr A1 A2, tarr B1 B2) :: H)).
+      { apply pair_env_valid_cons;
+          [now apply ValidTy_arr|now apply ValidTy_arr|exact VH]. }
+      apply IA.ia_WtPair.
+      * eapply build_certificate_bundle_annot_typing; eauto.
+        apply IA.ia_WtProj1. exact Hself.
+      * eapply build_certificate_bundle_annot_typing; eauto.
+        apply IA.ia_WtProj2. exact Hself.
+    + apply ValidTy_invert_prod in VA as [VA1 VA2].
+      apply ValidTy_invert_prod in VB as [VB1 VB2].
+      assert (VH' : PairEnvValid ((tprod A1 A2, tprod B1 B2) :: H)).
+      { apply pair_env_valid_cons;
+          [now apply ValidTy_prod|now apply ValidTy_prod|exact VH]. }
+      apply IA.ia_WtPair.
+      * eapply build_certificate_bundle_annot_typing; eauto.
+        apply IA.ia_WtProj1. exact Hself.
+      * eapply build_certificate_bundle_annot_typing; eauto.
+        apply IA.ia_WtProj2. exact Hself.
+    + apply ValidTy_invert_sum in VA as [VA1 VA2].
+      apply ValidTy_invert_sum in VB as [VB1 VB2].
+      assert (VH' : PairEnvValid ((tsum A1 A2, tsum B1 B2) :: H)).
+      { apply pair_env_valid_cons;
+          [now apply ValidTy_sum|now apply ValidTy_sum|exact VH]. }
+      apply IA.ia_WtPair.
+      * eapply build_certificate_bundle_annot_typing; eauto.
+        apply IA.ia_WtProj1. exact Hself.
+      * eapply build_certificate_bundle_annot_typing; eauto.
+        apply IA.ia_WtProj2. exact Hself.
+    + assert (VU : ValidTy body[beta1 (trec body)])
+        by now apply ValidTy_unfold_trec.
+      assert (VH' : PairEnvValid ((trec body, B) :: H))
+        by now apply pair_env_valid_cons.
+      eapply build_certificate_bundle_annot_typing; eauto.
+    + assert (VU : ValidTy body[beta1 (trec body)])
+        by now apply ValidTy_unfold_trec.
+      assert (VH' : PairEnvValid ((A, trec body) :: H))
+        by now apply pair_env_valid_cons.
+      eapply build_certificate_bundle_annot_typing; eauto.
+Qed.
+
+Lemma global_bundle_functional_annot_typing {Gamma A B}
+    (d : ClosedCastEq A B) :
+  ValidTy A -> ValidTy B ->
+  IA.AnnotTyping Gamma (global_bundle_functional_annot d)
+    (tarr (tarr tunit (certificate_bundle_ty d))
+      (tarr tunit (certificate_bundle_ty d))).
+Proof.
+  intros VA VB. unfold global_bundle_functional_annot.
+  assert (VBT : ValidTy (certificate_bundle_ty d)).
+  { eapply certificate_bundle_ty_valid; eauto using pair_env_valid_nil. }
+  apply IA.ia_WtAbs.
+  - apply ValidTy_arr;
+      [eauto with tyvalid cty simple_contr_rec|exact VBT].
+  - apply IA.ia_WtAbs.
+    + eauto with tyvalid cty simple_contr_rec.
+    + eapply build_certificate_bundle_annot_typing.
+      * apply pair_env_valid_nil.
+      * exact VA.
+      * exact VB.
+      * eapply IA.ia_WtApp.
+        -- apply IA.ia_WtVar. constructor. constructor.
+        -- apply IA.ia_WtUnit.
+      * apply cast_terms_annot_typing_nil.
+Qed.
+
+Theorem tied_certificate_bundle_annot_typing {Gamma A B}
+    (d : ClosedCastEq A B) :
+  ValidTy A -> ValidTy B ->
+  IA.AnnotTyping Gamma (tied_certificate_bundle_annot d)
+    (certificate_bundle_ty d).
+Proof.
+  intros VA VB. unfold tied_certificate_bundle_annot.
+  assert (VBT : ValidTy (certificate_bundle_ty d)).
+  { eapply certificate_bundle_ty_valid; eauto using pair_env_valid_nil. }
+  eapply IA.ia_WtApp.
+  - eapply IA.ia_WtApp.
+    + apply ufix_annot_typing.
+      * eauto with tyvalid cty simple_contr_rec.
+      * exact VBT.
+    + now apply global_bundle_functional_annot_typing.
+  - apply IA.ia_WtUnit.
+Qed.
+
+Theorem compile_global_pair_annot_typing {Gamma A B}
+    (d : ClosedCastEq A B) :
+  ValidTy A -> ValidTy B ->
+  IA.AnnotTyping Gamma (compile_global_pair_annot d) (cast_pair_ty A B).
+Proof.
+  intros VA VB. unfold compile_global_pair_annot.
+  apply certificate_root_annot_typing.
+  - now apply tied_certificate_bundle_annot_typing.
+  - apply cast_terms_annot_typing_nil.
+Qed.
+
+Theorem compile_global_up_annot_typing {Gamma A B}
+    (d : ClosedCastEq A B) :
+  ValidTy A -> ValidTy B ->
+  IA.AnnotTyping Gamma (compile_global_up_annot d) (tarr A B).
+Proof.
+  intros VA VB. apply pair_up_annot_typing.
+  now apply compile_global_pair_annot_typing.
+Qed.
+
+Theorem compile_global_down_annot_typing {Gamma A B}
+    (d : ClosedCastEq A B) :
+  ValidTy A -> ValidTy B ->
+  IA.AnnotTyping Gamma (compile_global_down_annot d) (tarr B A).
+Proof.
+  intros VA VB. apply pair_down_annot_typing.
+  now apply compile_global_pair_annot_typing.
+Qed.
