ExactBacktranslation/ExactCompiler.v
@@ -7,9 +7,11 @@ Require Import CompilerIE.Compiler.
 Require Import StlcEqui.SpecAnnot.
 Require Import StlcEqui.SpecEquivalent.
 Require StlcIso.SpecEquivalent.
+Require StlcIso.SpecAnnot.
 
 Module EAC := StlcEqui.SpecAnnot.
 Module CIEC := CompilerIE.Compiler.
+Module IAC := StlcIso.SpecAnnot.
 
 Lemma erase_equi_to_indexed_raw {Gamma t A} :
   EAC.AnnotTyping Gamma t A ->
@@ -34,9 +36,10 @@ Qed.
 Theorem exact_equi_annot_roundtrip {t A} :
   EAC.AnnotTyping empty t A ->
   StlcEqui.SpecEquivalent.PCtxEquivalent empty
-    (CIEC.compie (compile_equi_annot A t)) (EAC.eraseAnnot t) A.
+    (CIEC.compie (IAC.eraseAnnot (compile_equi_annot A t)))
+    (EAC.eraseAnnot t) A.
 Proof.
-  intros Ht. unfold compile_equi_annot.
+  intros Ht. rewrite erase_compile_equi_annot.
   pose proof (exact_equi_roundtrip (equi_to_indexed_typing Ht)) as Hround.
   now rewrite (erase_equi_to_indexed_raw Ht) in Hround.
 Qed.
@@ -48,13 +51,14 @@ Theorem exact_equi_annot_context_backtranslation {t C A R} :
   EAC.PCtxTypingAnnot empty A empty C R ->
   StlcEqui.SpecEquivalent.PCtxEquivalent empty
     (CIEC.compie
-      (StlcIso.SpecSyntax.pctx_app (compile_equi_annot A t)
-        (compile_equi_context_annot R C)))
+      (StlcIso.SpecSyntax.pctx_app
+        (IAC.eraseAnnot (compile_equi_annot A t))
+        (IAC.eraseAnnot_pctx (compile_equi_context_annot R C))))
     (StlcEqui.SpecSyntax.pctx_app (EAC.eraseAnnot t)
       (EAC.eraseAnnot_pctx C)) R.
 Proof.
   intros Ht HC.
-  unfold compile_equi_annot, compile_equi_context_annot.
+  rewrite erase_compile_equi_annot, erase_compile_equi_context_annot.
   pose proof (exact_indexed_context_backtranslation
     (equi_to_indexed_typing Ht)
     (equi_context_to_indexed_typing HC)) as Hround.
@@ -69,9 +73,10 @@ Theorem exact_equi_annot_full_abstraction {t1 t2 A} :
   (StlcEqui.SpecEquivalent.PCtxEquivalent empty
       (EAC.eraseAnnot t1) (EAC.eraseAnnot t2) A <->
    StlcIso.SpecEquivalent.PCtxEquivalent empty
-      (compile_equi_annot A t1) (compile_equi_annot A t2) A).
+      (IAC.eraseAnnot (compile_equi_annot A t1))
+      (IAC.eraseAnnot (compile_equi_annot A t2)) A).
 Proof.
-  intros Ht1 Ht2. unfold compile_equi_annot.
+  intros Ht1 Ht2. rewrite !erase_compile_equi_annot.
   pose proof (exact_indexed_full_abstraction
     (equi_to_indexed_typing Ht1)
     (equi_to_indexed_typing Ht2)) as Hfa.
