ExactBacktranslation/IndexedCompilerTests.v
@@ -2,9 +2,13 @@ Require Import ExactBacktranslation.IndexedCompiler.
 Require Import ExactBacktranslation.StructuralCoercionTests.
 Require Import ExactBacktranslation.StructuralCoercions.
 Require Import ExactBacktranslation.GlobalCoercions.
+Require Import ExactBacktranslation.AnnotatedGlobalCoercions.
 Require Import ExactBacktranslation.CertificateIndexedTests.
 Require Import StlcIso.SpecTyping.
+Require Import StlcIso.SpecAnnot.
 Require Import StlcEqui.SpecAnnot.
+
+Module IATest := StlcIso.SpecAnnot.
 
 Definition indexed_cyclic_cast_var : ICTm :=
   ic_coerce cycle_t_i cycle_s_i cyclic_cast_i (ic_var 0).
@@ -22,6 +26,18 @@ Example indexed_cyclic_compiler_output_typed :
   ⟪ empty r▻ cycle_t_i i⊢ compile_indexed indexed_cyclic_cast_var : cycle_s_i ⟫.
 Proof. exact (compile_indexed_typing indexed_cyclic_cast_var_typing). Qed.
 
+Example indexed_cyclic_annotated_compiler_output_typed :
+  IATest.AnnotTyping (empty r▻ cycle_t_i)
+    (compile_indexed_annot indexed_cyclic_cast_var) cycle_s_i.
+Proof.
+  exact (compile_indexed_annot_typing indexed_cyclic_cast_var_typing).
+Qed.
+
+Example indexed_cyclic_annotation_erases_to_raw_compiler :
+  IATest.eraseAnnot (compile_indexed_annot indexed_cyclic_cast_var) =
+  compile_indexed indexed_cyclic_cast_var.
+Proof. apply erase_compile_indexed_annot. Qed.
+
 Example indexed_cyclic_certificate_erasure_typed :
   ⟪ empty r▻ cycle_t_i ea⊢
       erase_indexed_certificate indexed_cyclic_cast_var : cycle_s_i ⟫.
@@ -32,4 +48,10 @@ Qed.
 Example indexed_cyclic_compilation_is_strict :
   compile_indexed indexed_cyclic_cast_var =
   I.app (compile_global_up cyclic_cast_i) (I.var 0).
+Proof. reflexivity. Qed.
+
+Example indexed_cyclic_annotated_compilation_is_strict :
+  compile_indexed_annot indexed_cyclic_cast_var =
+  IATest.ia_app cycle_t_i cycle_s_i
+    (compile_global_up_annot cyclic_cast_i) (IATest.ia_var 0).
 Proof. reflexivity. Qed.
